theories/Logic/MemInj.v
@@ -1,63 +1,45 @@
 From RSL Require Import Prelude.
 
-From RSL.Commons Require Export BijSet.
 From RSL.Logic Require Export PointsTo.
+From RSL.Commons Require Export BijSet.
 
-Definition related (j: gset (loc * loc)) (lt ls: loc) :=
-  (ls, lt) ∈ j.
+From RSL.Commons Require Import RegisterBank.
 
-Definition same_val (j: gset (loc * loc)) := val_eq (related j).
+Implicit Types (I E : gset (loc * loc)) (lt ls : loc).
 
-Lemma same_val_mono j j' vt vs :
-  j ⊆ j' ->
-  same_val j vt vs ->
-  same_val j' vt vs.
+Definition related I lt ls := (ls, lt) ∈ I.
+
+Definition same_val I := val_eq (related I).
+
+Definition regbank_same I (ρ1: regbank) (r1: reg) (ρ2: regbank) (r2: reg) :=
+  ∃ v1 v2,
+    ρ1@r1 ⇒ v1 ∧
+    ρ2@r2 ⇒ v2 ∧
+    same_val I v1 v2.
+
+Notation "ρ1 @ r1 '<{' I '}>' ρ2 @ r2" :=
+  (regbank_same I ρ1 r1%nat ρ2 r2%nat)
+    (at level 60, ρ2 at next level, no associativity).
+
+Lemma same_val_mono I I' vt vs :
+  I ⊆ I' ->
+  same_val I vt vs ->
+  same_val I' vt vs.
 Proof using Type.
   destruct vt as [], vs as []; simpl; auto.
   unfold related. by auto.
 Qed.
 
-Definition in_inj (j : gset (loc * loc)) (E: gmap loc loc) :=
-  ∀ ls lt, E !! ls = Some lt -> (ls, lt) ∈ j.
-
-Lemma in_inj_mono j j' E : j ⊆ j' -> in_inj j E -> in_inj j' E.
-Proof using Type.
-  by intros Hincl Hinj lt ls H; auto.
-Qed.
-
-Lemma in_inj_extend j E lt ls :
-  related j lt ls ->
-  in_inj j E ->
-  in_inj j (<[ls:=lt]> E).
-Proof using Type.
-  intros Hrel Hinj ls' lt'.
-  rewrite lookup_insert.
-  case_decide as He.
-  - intros H. by inv H.
-  - intros HeE. by apply Hinj.
-Qed.
-
-Lemma in_inj_remove j E ls :
-  in_inj j E ->
-  in_inj j (delete ls E).
-Proof using Type.
-  intros Hinj ls' lt'.
-  rewrite lookup_delete.
-  case_decide as He.
-  - intros H. by inv H.
-  - intros HeE. by apply Hinj.
-Qed.
-
-Definition mem_inj (j : gset (loc * loc)) (E: gmap loc loc) : rProp :=
+Definition mem_inj I E : rProp :=
   (
-    ⌜bij_set j⌟ ∗
-    ⌜in_inj j E⌟ ∗
-    [∗ set] '(ls, lt) ∈ j,
-      ∃ vt vs,
-        ⌜same_val j vt vs⌟ ∗
-        if (E !! ls)
+    ⌜bij_set I⌟ ∗
+    ⌜E ⊆ I⌟ ∗
+    [∗ set] '(ls, lt) ∈ I,
+        if (decide (ls ∈ dom E))
         then emp
-        else lt →ₜ vt ∗ ls →ₛ vs
+        else
+          ∃ vt vs,
+            ⌜same_val I vt vs⌟ ∗ lt →ₜ vt ∗ ls →ₛ vs
   )%I.
 
 Lemma inj_empty : ⊢ mem_inj ∅ ∅.
@@ -70,33 +52,39 @@ Proof using Type.
   { by iApply big_sepS_empty. }
 Qed.
 
-Lemma inj_insert_exploit j E lt ls vt vs :
-  E !! ls = None ->
-  (∀ ls' lt', E !! ls' = Some lt' -> lt' ≠ lt) ->
-  mem_inj j E -∗
+Lemma inj_insert_exploit I E lt ls vt vs :
+  ls ∉ dom E ->
+  lt ∉ codom E ->
+  mem_inj I E -∗
   lt →ₜ vt -∗
   ls →ₛ vs -∗
-  ⌜same_val j vt vs⌟ -∗
-  mem_inj ({[ (ls, lt) ]} ∪ j) E.
+  ⌜same_val I vt vs⌟ -∗
+  mem_inj ({[ (ls, lt) ]} ∪ I) E.
 Proof using Type.
   iIntros (Hls Hlt) "(%Hbij & %HE & Hin) Ht Hs %H".
 
-  iAssert (⌜∀ lt', (ls, lt') ∉ j⌝)%I with "[Hin Hs]" as "%Hs".
+  iAssert (⌜∀ lt', (ls, lt') ∉ I⌝)%I with "[Hin Hs]" as "%Hs".
   {
     iIntros (lt' Hej).
     iDestruct (big_sepS_delete _ _ _ Hej with "Hin") as "[Hcond H]".
-    rewrite Hls.
+    rewrite decide_False; last done.
     iDestruct "Hcond" as (vt' vs') "(_ & Ht' & Hs')".
     by iDestruct (src_points_to_unique with "Hs Hs'") as "%Hneq".
   }
 
-  iAssert (⌜∀ ls', (ls', lt) ∉ j⌝)%I with "[Hin Ht]" as "%Ht".
+  iAssert (⌜∀ ls', (ls', lt) ∉ I⌝)%I with "[Hin Ht]" as "%Ht".
   {
     iIntros (ls' Hej).
     iDestruct (big_sepS_delete _ _ _ Hej with "Hin") as "[Hcond H]".
-    destruct (E !! ls') as [lt'| ] eqn:HeE.
-    - assert (lt = lt'). { by eapply bij_set_functional; eauto. }
-      subst lt'. exfalso. by eapply Hlt.
+    case_decide as He.
+    - apply dom_spec in He as [lt' Hlt'].
+      assert (Heq: lt = lt').
+      { eapply bij_set_functional.
+        - by apply Hbij.
+        - by apply Hej.
+        - by apply HE.
+      }
+      subst lt. exfalso. apply Hlt. apply codom_spec. by eexists.
     - iDestruct "Hcond" as (vt' vs') "(_ & Ht' & Hs')".
       by iDestruct (tgt_points_to_unique with "Ht Ht'") as "%Hneq".
   }
@@ -104,85 +92,116 @@ Proof using Type.
   iSplitR.
   { iPureIntro. by apply bij_set_extend. }
   iSplitR.
-  { iPureIntro. apply in_inj_mono with j; auto. by apply union_subseteq_r. }
+  { iPureIntro. transitivity I; auto. by apply union_subseteq_r. }
   iApply big_sepS_union.
   { intros [] He%elem_of_singleton Hj. inv He. by apply (Ht ls). }
   iSplitR "Hin".
-  - iApply big_sepS_singleton. rewrite Hls.
+  - iApply big_sepS_singleton. rewrite decide_False; last done.
     iExists vt, vs. iFrame. iPureIntro.
-    apply same_val_mono with j; auto.
-    by apply union_subseteq_r.
+    apply same_val_mono with I.
+    + by apply union_subseteq_r.
+    + done.
   - iApply (big_sepS_impl with "Hin").
-    iModIntro. iIntros ([lt'' ls''] Hin) "(%vt' & %vs' & %Hsame & Hcond)".
-    iExists vt', vs'. iFrame.
-    iPureIntro.
-    apply same_val_mono with j; auto.
-    by apply union_subseteq_r.
+    iModIntro. iIntros ([lt'' ls''] Hin).
+    case_decide.
+    + by iIntros "$".
+    + iIntros "(%vt' & %vs' & %Hsame & Hcond)".
+      iExists vt', vs'. iFrame.
+      iPureIntro.
+      apply same_val_mono with I.
+      * by apply union_subseteq_r.
+      * done.
 Qed.
 
-Lemma inj_insert j lt ls vt vs :
-  mem_inj j ∅ -∗
+Lemma inj_insert I lt ls vt vs :
+  mem_inj I ∅ -∗
   lt →ₜ vt -∗
   ls →ₛ vs -∗
-  ⌜same_val j vt vs⌟ -∗
-  mem_inj ({[ (ls, lt) ]} ∪ j) ∅.
+  ⌜same_val I vt vs⌟ -∗
+  mem_inj ({[ (ls, lt) ]} ∪ I) ∅.
 Proof using Type. by apply inj_insert_exploit. Qed.
 
-Lemma inj_exploit j E lt ls :
-  related j lt ls ->
-  E !! ls = None ->
-  mem_inj j E -∗
+Lemma inj_exploit I E lt ls :
+  related I lt ls ->
+  ls ∉ dom E ->
+  mem_inj I E -∗
   ∃ vt vs,
     lt →ₜ vt ∗
     ls →ₛ vs ∗
-    ⌜same_val j vt vs⌟ ∗
-    mem_inj j (<[ls := lt]>E).
+    ⌜same_val I vt vs⌟ ∗
+    mem_inj I ({[ (ls, lt) ]} ∪ E).
 Proof using Type.
   iIntros (Hrel HnE) "(%Hbij & %HE & Hin)".
   iDestruct (big_sepS_delete _ _ _ Hrel with "Hin") as "[Hpair Hin]".
-  iDestruct "Hpair" as (vt vs) "[%Hsame Hcond]".
-  rewrite HnE.
-  iDestruct "Hcond" as "[Ht Hs]".
+  rewrite decide_False; last done.
+  iDestruct "Hpair" as (vt vs) "(%Hsame & Ht & Hs)".
   iExists vt, vs. iFrame.
   iSplitR. { done. }
 
   iSplitR. { done. }
-  iSplitR. { iPureIntro. by apply in_inj_extend. }
-
+  iSplitR.
+  { iPureIntro. apply union_subseteq. split.
+    - by apply elem_of_subseteq_singleton.
+    - easy.
+  }
   iApply (big_sepS_delete _ _ _ Hrel).
   iSplitR.
-  - iExists vt, vs. by rewrite lookup_insert decide_True.
+  - rewrite decide_True; first done.
+    apply dom_spec. eexists.
+    by apply elem_of_union_l, elem_of_singleton.
   - iApply (big_sepS_impl with "Hin").
     iModIntro.
     iIntros ([ls' lt'] Hneq).
-    iIntros "(%vt' & %vs' & Hsame & Hcond)".
-    iExists vt', vs'. iFrame.
     assert (ls ≠ ls') by (by eapply bij_set_diff_fst_neq).
-    now rewrite lookup_insert_ne.
+    case_decide as He.
+    + iIntros "_". rewrite decide_True; first done.
+      apply dom_union. by right.
+    + iIntros "(%vt' & %vs' & Hsame & Hcond)".
+      rewrite decide_False; first iFrame.
+      intros [->%dom_singleton | HinE]%dom_union; contradiction.
 Qed.
 
-Lemma inj_release j E lt ls vt vs:
-  E !! ls = Some lt ->
-  same_val j vt vs ->
-  mem_inj j E -∗
+Lemma inj_release I E lt ls vt vs:
+  (ls, lt) ∈ E ->
+  same_val I vt vs ->
+  mem_inj I E -∗
   lt →ₜ vt -∗
   ls →ₛ vs -∗
-  mem_inj j (delete ls E).
+  mem_inj I (E ∖ {[ (ls, lt) ]}).
 Proof using Type.
   iIntros (HE Hsame) "(%Hbij & %Hinj & Hin) Ht Hs".
   iSplitR. { done. }
-  iSplitR. { iPureIntro. by apply in_inj_remove. }
-  assert (Hin: (ls, lt) ∈ j) by (now apply Hinj).
+  iSplitR.
+  { iPureIntro. by apply subseteq_difference_l. }
+  assert (Hin: (ls, lt) ∈ I) by (now apply Hinj).
   iDestruct (big_sepS_delete _ _ _ Hin with "Hin") as "[H Hin]".
-  rewrite HE.
-  iDestruct "H" as (vt' vs' Hsame') "_".
   iApply (big_sepS_delete _ _ _ Hin).
   iSplitL "Ht Hs".
-  - iExists vt, vs. rewrite lookup_delete_eq. by iFrame.
-  - iApply (big_sepS_impl with "Hin"). clear vt' vs' Hsame'.
+  { rewrite decide_False.
+    - iExists vt, vs. by iFrame.
+    - intros [lt' [Hin' HnIn]%elem_of_difference]%dom_spec.
+      apply HnIn, elem_of_singleton. f_equal.
+      by eapply bij_set_functional; eauto. }
+  iApply (big_sepS_impl with "Hin").
+  rewrite decide_True.
+  - iDestruct "H" as "_".
     iModIntro.
-    iIntros ([ls' lt'] Hin') "(%vt' & %vs' & Hsame & H)".
-    iExists vt', vs'. iFrame.
+    iIntros ([ls' lt'] Hin').
     assert (ls ≠ ls') by (by eapply bij_set_diff_fst_neq).
-    now rewrite lookup_delete_ne.
+    case_decide as He.
+    + iIntros "_".
+      rewrite decide_True; first done.
+      apply dom_spec in He as [lt'' He].
+      apply dom_spec. exists lt''.
+      apply elem_of_difference. split; first done.
+      intros Hcontra%elem_of_singleton.
+      inv Hcontra.
+    + iIntros "(%vt' & %vs' & Hsame & H)".
+      rewrite decide_False; first iFrame.
+      intros Hcontra.
+      apply He.
+      apply dom_spec in Hcontra as [y Hinc].
+      apply elem_of_difference in Hinc as [].
+      apply dom_spec. by exists y.
+  - apply dom_spec. by eexists.
 Qed.
