theories/Playground/SimTest.v
@@ -1,0 +1,229 @@
+From RSL Require Import Prelude.
+
+From RSL.Logic Require Import Logic.
+From RSL.RTL Require Import SimRules.
+
+Import RTLNotations.
+
+Section T.
+  Let Λₜ : lang := rtl_lang.
+  Let Λₛ : lang := rtl_lang.
+  Context (Pₜ : prog Λₜ) (Pₛ : prog Λₛ).
+
+  Abbreviation fsim := (fsim WfNat WfNat Pₜ Pₛ).
+
+  Let reg_n : reg := 1.
+  Let reg_res : reg := 2.
+  Let reg_one : reg := 3.
+  Let reg_addr : reg := 4.
+  Let reg_cond : reg := 5.
+
+  Definition fact_bad : function :=
+    {|
+      fn_name := "fact"%string;
+      fn_regs := [reg_n; reg_addr];
+      fn_entrypoint := 0;
+      fn_code :=
+        <<{{
+              0: reg_res := #(VInt 1) -> 1;
+              1: !reg_addr := reg_res -> 2;
+              2: reg_cond := isZ reg_n -> 3;
+              3: if reg_cond then goto 7 else goto 4;
+              4: reg_res := reg_res * reg_n -> 5;
+              5: reg_one := !reg_addr -> 6;
+              6: reg_n := reg_n - reg_one -> 2;
+              7: ret reg_res;
+          }}>>;
+      fn_regs_no_dup := eq_refl;
+    |}.
+
+  Definition fact_good : function :=
+    {|
+      fn_name := "fact"%string;
+      fn_regs := [reg_n; reg_addr];
+      fn_entrypoint := 0;
+      fn_code :=
+        <<{{
+              0: reg_res := #(VInt 1) -> 1;
+              1: !reg_addr := reg_res -> 2;
+              2: reg_one := #(VInt 1) -> 3;
+              3: reg_cond := isZ reg_n -> 4;
+              4: if reg_cond then goto 7 else goto 5;
+              5: reg_res := reg_res * reg_n -> 6;
+              6: reg_n := reg_n - reg_one -> 3;
+              7: ret reg_res;
+        }}>>;
+      fn_regs_no_dup := eq_refl;
+    |}.
+
+  Notation
+    "'[' C ']' st '<{' j ',' i '}=' ss '{{' Q '}}'" :=
+    (sim_lfp Pₜ Pₛ C st j i ss Q%I)
+      (at level 0,
+       st at level 99,
+       ss at level 99,
+       Q at level 200,
+       no associativity).
+
+  Ltac close_hyp :=
+    match goal with
+    | [ |- ?f @ ?pc is _] => done
+    | [ |- ?ρ @ ?l ⇒ _ ] => try simregs
+    | [ |- eval_op ?op ?vals = Some _ ] => done
+    | [ |- (if _ then _ else _) = _ ] => done
+    | [ |- context [(_ →ₜ _)%I] ] => try iAssumption
+    | [ |- context [(_ →ₛ _)%I] ] => try iAssumption
+    | [ |- context [mem_inj _ _] ] => try iAssumption
+    | [ |- same_val _ _ _ ] => try done
+    | [ |- ?goal ] => idtac
+    end.
+
+  Definition samer I vt vs : rProp :=
+    ∃ I',
+      ⌜same_val I vt vs⌟ ∗
+      ⌜I ⊆ I'⌟ ∗
+      mem_inj I' ∅.
+
+  Local Definition inv lt ls v (st: pstate Λₜ) (j i: nat) (ss: pstate Λₛ) ψ : rProp :=
+    ∃ I ρt ρs,
+      mem_inj I {[ (ls, lt) ]} ∗
+      ls →ₛ v ∗
+      lt →ₜ v ∗
+      (∀ vt vs, samer I vt vs -∗ ψ vt vs) ∗
+      ⌜
+        st = ([], State fact_good 3 ρt) ∧
+        ss = ([], State fact_bad 2 ρs) ∧
+        ρt @ reg_n <{ I }> ρs @ reg_n ∧
+        ρt @ reg_res <{ I }> ρs @ reg_res ∧
+        ρt @ reg_one ⇒ v ∧
+        ρs @ reg_addr ⇒ VPtr ls ∧
+        ρt @ reg_addr ⇒ VPtr lt
+      ⌟.
+
+  Lemma fact_same C I :
+    ∀ args_t args_s,
+    Forall2 (same_val I) args_t args_s ->
+    mem_inj I ∅ -∗
+    [C]
+      ([], CallState fact_good args_t)
+        <{0, 0}=
+      ([], CallState fact_bad args_s)
+    {{ samer I }}.
+  Proof using Type.
+    intros args_t args_s Hsame.
+    iIntros "Hinj".
+    iApply (source_callstate_exploit).
+    iIntros (ρs pc Hlen -> ->).
+    iApply (target_callstate); [ by eapply Forall2_length_r | done | done |].
+
+    destruct (init_regs_sound fact_bad args_s) as (ρs & <- & Hs).
+    { done. }
+
+    destruct (init_regs_sound fact_good args_t) as (ρt & <- & Ht).
+    { by eapply Forall2_length_r. }
+
+    destruct args_s as [|vs_n [|vs_addr []]]; inv Hlen.
+    apply Forall2_cons_inv_r in Hsame as (vt_n & ? & Hv & Hsame & ->).
+    apply Forall2_cons_inv_r in Hsame as (vt_addr & ? & Hreg & Hsame & ->).
+    apply Forall2_nil_inv_r in Hsame as ->.
+
+    eassert (ρs@reg_n ⇒ _) by (by apply Hs with 0).
+    eassert (ρt@reg_n ⇒ _) by (by apply Ht with 0).
+
+    eassert (ρs@reg_addr ⇒ _) by (by apply Hs with 1).
+    eassert (ρt@reg_addr ⇒  _) by (by apply Ht with 1).
+
+    clear Ht Hs.
+
+    iApply (source_op). all: close_hyp.
+    iApply (target_op). all: close_hyp.
+    simpl.
+
+    iApply (source_store_exploit). all: close_hyp.
+    { by set_solver. }
+    iIntros (lt ls vt -> ->).
+    iIntros "Ht Hs Hinj".
+
+    iApply (target_store with "[-Ht] Ht"). all: close_hyp.
+    iIntros "Ht".
+    simpl.
+
+    iApply (target_op). all: close_hyp.
+    simpl.
+
+    iApply (coind Pₜ Pₛ C (inv lt ls (VInt 1))).
+    {
+      clear.
+      iIntros "!>" (C st j i ss ϕ) "#CIH".
+      iIntros "(%I & %ρt & %ρs & Hinj & Hs & Ht & Hpost & %Hinv)".
+      destruct Hinv as (-> & -> & Hn & Hres & Hone & Haddr_s & Haddr_t).
+
+      destruct Hn as (vn_t & vn_s & ? & ? & Hsame_n).
+      destruct Hres as (vres_t & vres_s & ? & ? & Hsame_res).
+      simpl.
+
+      iApply (source_op_exploit). all: close_hyp.
+      iIntros (v Hz).
+      destruct vn_s as [ vn | | | ], vn_t; inv Hz; inv Hsame_n.
+
+      iApply (target_op). all: close_hyp.
+      simpl.
+
+      iApply (source_if). all: close_hyp.
+      iApply (target_if). all: close_hyp.
+      simpl.
+
+      destruct (vn =? 0)%Z.
+      - iApply (source_ret). all: close_hyp.
+        iApply (target_ret). all: close_hyp.
+        iApply (both_final).
+        iAssert (mem_inj I ∅) with "[Hinj Ht Hs]" as "Hinj".
+        {
+          replace ∅ with ({[(ls, lt)]} ∖ {[(ls, lt)]} : gset (loc * loc)) by set_solver.
+          iApply (inj_release with "Hinj Ht Hs"); by set_solver.
+        }
+        iApply "Hpost".
+        iExists I. iFrame. by iPureIntro.
+      -
+        iApply (source_op_exploit). all: close_hyp.
+        iIntros (? Hv).
+        destruct vres_s, vres_t; inv Hv; inv Hsame_res.
+
+        iApply (target_op). all: close_hyp.
+        simpl.
+
+        iApply (source_load with "[-Hs] [Hs]"). all: close_hyp.
+        iIntros "Hs".
+
+        iApply (source_op). all: close_hyp.
+        iApply (target_op). all: close_hyp.
+        simpl.
+
+        iApply "CIH"; try (iPureIntro; by lia).
+        iExists I, _, _. iFrame. iPureIntro.
+        split_and!.
+        + reflexivity.
+        + reflexivity.
+        + eexists _, _. split_and!; simregs || done.
+        + eexists _, _. split_and!; simregs || done.
+        + simregs.
+        + simregs.
+        + simregs.
+    }
+    replace ({[(ls, lt)]} ∪ ∅) with ({[(ls, lt)]} : gset (loc * loc)) by set_solver.
+    iExists I, _, _. iFrame.
+    iSplit. { by iIntros (? ?) "$". }
+    iPureIntro. split_and!.
+    - reflexivity.
+    - reflexivity.
+    - eexists _, _. split_and!; simregs || done.
+    - eexists _, _. split_and!; simregs || done.
+    - simregs.
+    - simregs.
+    - simregs.
+  Qed.
+End T.
+
+(* Memcopy avec déroulage de boucle ? *)
+(* Optimisations des nop ? *)
+(* Inlining à la main ? *)
